Simpler invariant without nesting and part of proof for LockServer.TryLock

src/program_proof/lockservice/proof.v
@@ -10,7 +10,7 @@ From Perennial.algebra Require Import auth_map fmcounter.
 From Perennial.goose_lang.lib Require Import lock.
 From Perennial.Helpers Require Import NamedProps.
 From iris.algebra Require Import numbers.
-
+From Coq.Structures Require Import OrdersTac.
 Section lockservice_proof.
 Context `{!heapG Σ}.
 
@@ -36,43 +36,6 @@ Record LockReplyC :=
   }.
 Instance: Settable LockReplyC := settable! mkLockReplyC <OK>.
 
-(*
-
-Having token Cache(CID, S, A) should mean that 
-the server has seen the seq number S, and responded with A (on a call to Lock).
-
-{ ??? } LockServer__TryLock {RET false; ok = true → (inv (P ∨ Token)) }
-The first time TryLock runs, it has P. Later on, it no longer has P, so it needs to get the invariant from somewhere.
-Need to know (first time running ∨ escrow_inv_holds)
-
-First time running iff the req.seq > lasSeq[CID]
-Owning a clerk -> ck.seq > lastSeq[ck.CID]
-Clerk has frag ownership of the last seq seen by the server.
-
-∃ ls_seq ck_seq, own ls_γ ◯E(ls_seq) ∧ own ck_γ (Excl ck_seq)
-(⌜ck_seq > ls_γ⌝ ∨ (resp for ck_seq is false) ∨ (inv (P ∨ Token)))
-
-own (resp_γ ck_cid ck_seq) (Agree false)
-
-If the first disjunct holds, then we can show that the reply cache doesn't have a response for the request.  Then, if TryLock replies true, then we have P and hence right disjunct. If TryLock replies false, we know that it will always reply false with the same input.
-
-Use an auth_map to keep track of the reply history.
-
-(ck_cid, ck_seq) [[rc_γ]]↦ false
-
-Invariant for CallTryLock looks like 
-∃ ls_seq ck_seq, own ls_γ ◯E(ls_seq) ∧ own ck_γ (F{1/2} ck_seq)
-(⌜ck_seq > ls_γ⌝ ∨ ((ck_cid, ck_seq) [[rc_γ]]↦ false) ∨ (inv (P ∨ Token)))
-
-Ghost state for server:
-(auth_map) ck_cid [[γ]]↦ (last_seq, last_reply)
-
-∃ ls_seq ck_seq last_reply, ∧ own ck_γ (F{1/2} ck_seq)
-(⌜ck_seq > ls_γ⌝ ∨ ⌜last_reply = false⌝ ∨ (inv (P ∨ Token))) ∗
-(ck_cid [[rc_γ]]↦ (ls_seq, last_reply) 
-*)
-
-Print into_val.IntoVal.
 Global Instance ToVal_bool : into_val.IntoVal bool.
 Proof.
   refine {| into_val.to_val := λ (x: bool), #x;
@@ -81,12 +44,14 @@ Defined.
 
 Definition locknameN (lockname : u64) := nroot .@ "lock" .@ lockname.
 
-
   Context `{!mapG Σ u64 (u64 * bool)}.
+  Context `{!mapG Σ u64 u64}.
+  Context `{!mapG Σ (u64*u64) (option bool)}.
   Context `{!inG Σ (exclR unitO)}.
   Context `{!inG Σ (gmapUR u64 fmcounterUR)}.
+  Context `{!inG Σ (gmapUR u64 (lebnizO boolO))}.
 
-Definition own_clerk (ck:val) (srv:val) (γ:gname) (rc_γ:gname) : iProp Σ
+Definition own_clerk (ck:val) (srv:val) (γ:gname) (rcγ:gname) : iProp Σ
   :=
   ∃ (ck_l:loc) (cid seq ls_seq : u64) (last_reply:bool),
     ⌜ck = #ck_l⌝
@@ -94,39 +59,55 @@ Definition own_clerk (ck:val) (srv:val) (γ:gname) (rc_γ:gname) : iProp Σ
     ∗ck_l ↦[Clerk.S :: "cid"] #cid
     ∗ck_l ↦[Clerk.S :: "cid"] #seq
     ∗ck_l ↦[Clerk.S :: "primary"] srv
-    ∗ (cid [[rc_γ]]↦ (ls_seq, last_reply))
+    ∗ (cid [[rcγ]]↦ (ls_seq, last_reply))
        (*∗own γ (seq) *)
 .
 
-Definition CallTryLock_inv (seq cid:u64) rc_ptsto_in_inv_γ lastSeq_γ rc_γ (P:iProp Σ) (Pγ:gname) (N:namespace) : iProp Σ :=
-  (  "Hrc_ptsto_in_inv" ∷ own rc_ptsto_in_inv_γ (Excl ())
-   ∗ "HseqTooSmall" ∷ own lastSeq_γ {[ cid := (◯MaxNat (int.nat seq)) ]})
-   ∨ 
-  (∃ (ls_seq:u64) (last_reply:bool),
-    (">Hrc_ptsto" ∷ cid [[rc_γ]]↦ (ls_seq, last_reply))
-      ∗ "HTryLockCases" ∷ (
-         ">Hcase" ∷ ⌜int.nat seq > int.nat ls_seq⌝
-         ∨ (">Hcase" ∷  ⌜seq = ls_seq ∧ last_reply = false⌝
-            ∗ own lastSeq_γ {[ cid := (◯MaxNat (int.nat seq)) ]})
-         ∨ ("Hcase" ∷  (inv N (P ∨ own Pγ (Excl ())))
-            ∗ own lastSeq_γ {[ cid := (◯MaxNat (int.nat seq)) ]})
-      )
-      )
+(* Either the request owns the lastSeq[cid] ptsto, or it
+knows that it won't need it by way of knowing that lastSeq[cid] >= seq *)
+Definition LockReq_inner (seq cid ln:u64) rcγ lseqγ req_owns_lseqγ (Ps:u64 -> iProp Σ) (Pγ:gname) : iProp Σ :=
+  "Hlseq_prop" ∷ ( (∃ lseq : u64,
+        ⌜int.nat lseq ≤ int.nat seq⌝ ∗
+         own lseqγ {[ cid := (●{1/2}MaxNat (int.nat lseq))]} 
+         ∗ (⌜int.nat lseq < int.nat seq⌝ ∨ (∃ (last_reply:bool), (cid, seq) [[rcγ]]↦ro Some last_reply
+                          ∗ ⌜lseq = seq⌝ ∗ (⌜last_reply = false⌝ ∨ (Ps ln) ∨ own Pγ (Excl ())))
+                   ))
+                   ∨
+                   (own req_owns_lseqγ (Excl ())) ∗ (own lseqγ {[ cid := (◯MaxNat (int.nat seq)) ]} )
+                 )
+(*
+  ∗
+  "Hrc_ptsto" ∷ (
+  (cid, seq) [[rcγ]]↦ None
+  ∨ (∃ (last_reply:bool), (cid, seq) [[rcγ]]↦ro Some last_reply
+  ∗ (own lseqγ {[ cid := (◯MaxNat (int.nat seq)) ]} ) ∗ (⌜last_reply = false⌝ ∨ (Ps ln) ∨ own Pγ (Excl ())))
+  )
+ *)
 .
 
-Definition own_lockserver (srv:loc) (rc_γ:gname) (Ps: u64 -> (iProp Σ)) : iProp Σ:=
+Definition own_lockserver (srv:loc) (rcγ:gname) (lseqγ:gname) (Ps: u64 -> (iProp Σ)) : iProp Σ:=
   ∃ (lastSeq_ptr lastReply_ptr locks_ptr:loc) (lastSeqM:gmap u64 u64)
-    (lastReplyM locksM:gmap u64 bool),
+    (lastReplyM locksM:gmap u64 bool) (replyHistory:gmap (u64*u64) (option bool)),
     (
       "HlastSeqOwn" ∷ srv ↦[LockServer.S :: "lastSeq"] #lastSeq_ptr
-    ∗ "HlastSeqMap" ∷ is_map (lastSeq_ptr) lastSeqM
     ∗ "HlastReplyOwn" ∷ srv ↦[LockServer.S :: "lastReply"] #lastReply_ptr
-    ∗ "HlastReplyMap" ∷ is_map (lastReply_ptr) lastReplyM
     ∗ "HlocksOwn" ∷ srv ↦[LockServer.S :: "locks"] #locks_ptr
+
+    ∗ "HlastSeqMap" ∷ is_map (lastSeq_ptr) lastSeqM
+    ∗ "HlastReplyMap" ∷ is_map (lastReply_ptr) lastReplyM
     ∗ "HlocksMap" ∷ is_map (locks_ptr) locksM
-    ∗ "Hmapctx" ∷ map_ctx rc_γ 1 (map_zip lastSeqM lastReplyM)
-    (* ∗ "HlastSeq_γ" ∷ own , *)
-    ∗ "HPs" ∷ [∗ map] ln ↦ held ∈ locksM, (⌜held=true⌝ ∨ (Ps ln))
+
+    ∗ ("Hrcctx" ∷ map_ctx rcγ 1 replyHistory)
+    ∗ ("Hownlseqγ" ∷ [∗ map] cid ↦ lseq ∈ lastSeqM, own lseqγ {[ cid := (●{1/2}MaxNat (int.nat lseq))]} )
+    ∗ ("#Hrc_lseqbound" ∷ [∗ map] cid_seq ↦ r ∈ replyHistory, own lseqγ {[ cid_seq.1 := (◯MaxNat (int.nat cid_seq.2))]} )
+
+    ∗ ("#Htbd" ∷ [∗ map] cid_seq ↦ r ∈ replyHistory,
+       ⌜r = None⌝ ∨ cid_seq [[rcγ]]↦ro r)
+
+    ∗ ("%" ∷ ⌜forall (cid seq:u64) r, lastSeqM !! cid = Some seq ∧ lastReplyM !! cid = Some r → replyHistory !! (cid, seq) = Some (Some r)⌝)
+    ∗ ("%" ∷ ⌜forall (cid seq:u64), lastSeqM !! cid = Some seq → (∃ r, lastReplyM !! cid = Some r)⌝)
+
+    ∗ "Hlockeds" ∷ [∗ map] ln ↦ locked ∈ locksM, (⌜locked=true⌝ ∨ (Ps ln))
     )%I
 .
 
@@ -141,24 +122,38 @@ Definition own_lock_reply (args_ptr:loc) (lockReply:LockReplyC): iProp Σ :=
   args_ptr ↦[LockReply.S :: "OK"] #lockReply.(OK)
 .
 
-Definition is_lockserver srv rc_γ Ps lockN: iProp Σ :=
+Definition is_lockserver srv rcγ lseqγ Ps lockN: iProp Σ :=
   ∃ (mu_ptr:loc),
-    readonly (srv ↦[LockServer.S :: "mu"] #mu_ptr)
-             ∗(is_lock lockN #mu_ptr (own_lockserver srv rc_γ Ps))
+    "Hmuptr" ∷ readonly (srv ↦[LockServer.S :: "mu"] #mu_ptr)
+             ∗ ( "Hmu" ∷ is_lock lockN #mu_ptr (own_lockserver srv rcγ lseqγ Ps))
 .
 
-Lemma TryLock_spec (srv args reply:loc) (lockArgs:LockArgsC) (lockReply:LockReplyC) rc_γ (Ps: u64 -> (iProp Σ)) P Pγ N M lockN:
+Instance inj_MaxNat_equiv : Inj eq equiv MaxNat.
+Proof.
+  intros n1 n2.
+  intros ?%leibniz_equiv.
+  inversion H0; auto.
+Qed.
+
+Lemma TryLock_spec (srv args reply:loc) (lockArgs:LockArgsC) (lockReply:LockReplyC) rcγ (lseqγ:gname) req_owns_lseqγ (Ps: u64 -> (iProp Σ)) P Pγ M lockN :
   Ps lockArgs.(Lockname) = P →
-  {{{ is_lockserver srv rc_γ Ps lockN∗inv M (CallTryLock_inv lockArgs.(Seq) lockArgs.(CID) rc_γ P Pγ N) ∗read_lock_args args lockArgs
-  ∗ own_lock_reply reply lockReply }}}
-    LockServer__TryLock #srv #args #reply
-  {{{ RET #false; ∃ ok, (⌜ok = true⌝∗(inv N (P ∨ own Pγ (Excl()))) ∨ ⌜ok = false⌝) ∗ reply ↦[LockReply.S :: "OK"] #ok }}}.
+  {{{ "#Hls" ∷ is_lockserver srv rcγ lseqγ Ps lockN
+      ∗ "#HargsInv" ∷ inv M (LockReq_inner lockArgs.(Seq) lockArgs.(CID) lockArgs.(Lockname) rcγ lseqγ req_owns_lseqγ Ps Pγ)
+      ∗ "#Hargs" ∷ read_lock_args args lockArgs
+      ∗ "Hreply" ∷ own_lock_reply reply lockReply
+      ∗ "Hcond_own" ∷ own req_owns_lseqγ (Excl ())
+  }}}
+LockServer__TryLock #srv #args #reply
+{{{ RET #false; ∃ (ok:bool), reply ↦[LockReply.S :: "OK"] #ok
+                                   ∗ (lockArgs.(CID), lockArgs.(Seq)) [[rcγ]]↦ro (Some ok)
+}}}.
 Proof.
   intros HPs.
-  iIntros (Φ) "(#Hls & #HinvM & Hargs & Hreply) HPost".
+  iIntros (Φ) "Hpre HPost".
+  iNamed "Hpre".
   wp_lam.
   wp_pures.
-  iDestruct "Hls" as (mu_ptr) "(Hls & Hmu)".
+  iNamed "Hls".
   wp_loadField.
   wp_apply (acquire_spec lockN #mu_ptr _ with "Hmu").
   iIntros "(Hlocked & Hlsown)".
@@ -171,50 +166,163 @@ Proof.
   iIntros (v ok) "(HSeqMapGet&HlastSeqMap)"; iDestruct "HSeqMapGet" as %HSeqMapGet.
   wp_pures.
   destruct ok.
-  - (* Case cid in lastSeqM *) admit.
-  - (* Case cid not in lastSeqM, so don't look at cache *)
-    wp_pures.
-    wp_loadField.
-    wp_loadField.
-    wp_loadField.
-    Check wp_MapInsert.
-    wp_apply (wp_MapInsert _ _ lastSeqM _ lockArgs.(Seq) (#lockArgs.(Seq)) with "HlastSeqMap"); try eauto.
-    iIntros "HlastSeqMap".
-    wp_pures.
-    wp_loadField.
-    wp_loadField.
-    wp_apply (wp_MapGet with "HlocksMap").
-    iIntros (lock_v ok) "(HLocksMapGet&HlocksMap)"; iDestruct "HLocksMapGet" as %HLocksMapGet.
-    wp_pures.
-    destruct lock_v.
-    + (* Lock already held by someone *)
-      wp_pures.
-      wp_storeField.
+  - (* Case cid in lastSeqM *)
+    apply map_get_true in HSeqMapGet.
+    wp_pures. repeat wp_loadField. wp_binop.
+    destruct bool_decide eqn:Hineq.
+    -- (* old seqno *)
+      apply bool_decide_eq_true in Hineq.
+      wp_pures. 
       repeat wp_loadField.
-      wp_apply (wp_MapInsert _ _ lastReplyM _ false #false with "HlastReplyMap"); first eauto; iIntros "HlastReplyMap".
+      wp_apply (wp_MapGet with "HlastReplyMap").
+      iIntros (reply_v reply_get_ok) "(HlastReplyMapGet & HlastReplyMap)"; iDestruct "HlastReplyMapGet" as %HlastReplyMapGet.
+      wp_storeField.
+      assert (reply_get_ok = true) as ->; first admit.
+      apply map_get_true in HlastReplyMapGet.
       iApply fupd_wp.
-      iInv "HinvM" as "HM" "HCloseM".
-      iDestruct "HM" as (ls_seq seq last_reply) "[Hptsto #HMM]".
-      iMod "Hptsto".
-      iMod (map_update lockArgs.(CID) (ls_seq, last_reply) (lockArgs.(Seq), false) with "Hmapctx Hptsto") as "(Hmapctx & Hptsto)".
-      rewrite (map_insert_zip_with pair _ _ lockArgs.(CID) _ _).
-      iMod ("HCloseM" with "[Hptsto]") as "_".
-      { iModIntro.
-        unfold CallTryLock_inv.
-        iExists lockArgs.(Seq).
-        admit. }
-      iModIntro.
-      wp_seq.
-      wp_loadField.
-      wp_apply (release_spec lockN #mu_ptr _ with "[-Hreply HPost]"); try iFrame "Hmu Hlocked".
-      { (* Estanlish own_lockserver *)
-        iNext. iFrame.
-        iExists _, _, _, _, _, _; iFrame.
+
+      (* Use invariant to get Hrc_ptsto, and know that its seqno matches the seqno in request *)
+      iInv M as "HMinner" "HMClose".
+      iDestruct "HMinner" as "Hlseq_prop".
+      iDestruct "Hlseq_prop" as "[Hlseq_prop|Hlseq_bad]"; last admit.
+      iDestruct "Hlseq_prop" as (real_lseq) "[#>Hle [>Hlseq_own Hcases]]".
+      iDestruct "Hle" as %Hle.
+      iDestruct (big_sepM_delete _ _ lockArgs.(CID) v with "Hownlseqγ") as "(Hlseq_frombigSep & Hlseqγauth)"; first done.
+      iCombine "Hlseq_own Hlseq_frombigSep" as "Hcombined".
+      iDestruct (own_valid with "Hcombined") as %Hvalid.
+      apply singleton_valid in Hvalid.
+      apply auth_auth_frac_op_inv in Hvalid.
+      symmetry in Hvalid.
+      apply (inj MaxNat) in Hvalid.
+      assert (v = real_lseq) as Htemp. {
+        replace (v) with (real_lseq) by word. done.
       }
-      wp_seq. iApply ("HPost").
-      iExists false. iFrame. by iRight.
-    + (* Lock not held by anyone *)
-      wp_pures. wp_storeField. repeat wp_loadField.
+      destruct Htemp.
+      destruct Hvalid.
+      iDestruct "Hcombined" as "[Hlseq_own Hlseq_frombigSep]".
+      iDestruct (big_sepM_delete _ _ lockArgs.(CID) v with "[$Hlseqγauth $Hlseq_frombigSep]") as "Hlseqγauth"; first done.
+      
+      assert (v = lockArgs.(Seq)) as ->; first admit. (* By inequalities *)
+      iDestruct (big_sepM_delete _ _ (lockArgs.(CID), lockArgs.(Seq)) (Some reply_v) with "Htbd") as "(#Hreply_prop & _)".
+      {
+        (* Using foralls *)
+        admit.
+      }
+      iMod ("HMClose" with "[Hlseq_own Hcases]") as "_".
+      { iNext. iLeft. iExists _; iFrame. iFrame "%". }
+      iModIntro.
+
+      iDestruct "Hreply_prop" as "[Hbad|Hrc_ptsto]".
+      { iDestruct "Hbad" as %Hbad; iExFalso; iPureIntro. discriminate Hbad. }
+      wp_loadField.
+      wp_apply (release_spec lockN #mu_ptr _ with "[-Hreply Hcond_own Hrc_ptsto HPost]"); try iFrame "Hmu Hlocked".
+      {
+        iNext. iExists _, _, _, _, _, _, _; try iFrame; try iFrame "#"; try iFrame "%".
+      }
+
+      wp_seq.
+      iApply "HPost".
+      iExists reply_v.
+      iFrame "#"; iFrame.
+    -- (* new seqno *)
+      apply bool_decide_eq_false in Hineq.
+      rename Hineq into HnegatedIneq.
+      assert (int.val lockArgs.(Seq) > int.val v)%Z as Hineq; first lia.
+      wp_pures.
+      wp_loadField.
+      wp_loadField.
+      wp_loadField.
+      Check wp_MapInsert.
+      wp_apply (wp_MapInsert _ _ lastSeqM _ lockArgs.(Seq) (#lockArgs.(Seq)) with "HlastSeqMap"); try eauto.
+      iIntros "HlastSeqMap".
+      wp_pures.
+      wp_loadField.
+      wp_loadField.
+      wp_apply (wp_MapGet with "HlocksMap").
+      iIntros (lock_v ok) "(HLocksMapGet&HlocksMap)"; iDestruct "HLocksMapGet" as %HLocksMapGet.
+      wp_pures.
+      destruct lock_v.
+      + (* Lock already held by someone *)
+        wp_pures.
+        wp_storeField.
+        repeat wp_loadField.
+        wp_apply (wp_MapInsert _ _ lastReplyM _ false #false with "HlastReplyMap"); first eauto; iIntros "HlastReplyMap".
+        wp_seq. wp_loadField.
+        iApply fupd_wp.
+        iInv M as "HMinner" "HMClose".
+        iDestruct "HMinner" as "[HMinner|Hbad]"; last admit.
+        iDestruct "HMinner" as (real_lseq) "[#>Hle [>Hlseq_own Hcases]]".
+        assert (v = real_lseq) as Htemp; first admit. (* TODO: make this a lemma *)
+        Check map_alloc.
+        iAssert ⌜replyHistory !! (lockArgs.(CID), lockArgs.(Seq)) = None⌝%I as %HtempMap.
+        {
+          admit.
+        }
+        iMod (map_alloc_ro (lockArgs.(CID), lockArgs.(Seq)) (Some false) with "Hrcctx") as "[Hrcctx #Hrc_ptsto]"; first done.
+        iDestruct (big_sepM_delete _ _ lockArgs.(CID) v with "Hownlseqγ") as "(Hlseq_frombigSep & Hlseqγauth)"; first done.
+        Check own_update_2.
+        destruct Htemp.
+        iCombine "Hlseq_frombigSep Hlseq_own" as "Hcombined".
+        iMod (own_update with "Hcombined") as "Hcombined".
+        {
+          eapply singleton_update.
+          eapply auth_update_alloc.
+          eapply (max_nat_local_update _ _ (MaxNat (int.nat lockArgs.(Seq)))). simpl. lia.
+        }
+        iDestruct "Hcombined" as "[[Hlseq_frombigSep Hlseq_own] Hfrag]".
+        iDestruct (big_sepM_insert_delete with "[$Hlseqγauth $Hlseq_frombigSep]") as "Hlseqγauth".
+        Check big_sepM_insert.
+        iDestruct (big_sepM_insert _ _ (lockArgs.(CID), lockArgs.(Seq)) _ with "[$Hrc_lseqbound $Hfrag]") as "#Hrc_lseqbound2"; first done.
+        iDestruct (big_sepM_insert _ _ (lockArgs.(CID), lockArgs.(Seq)) _ with "[$Htbd $Hrc_ptsto]") as "#Htbd2"; first done.
+        
+        iMod ("HMClose" with "[Hrc_ptsto Hcases Hlseq_own]") as "_".
+        { iNext. iLeft. iExists _; iFrame. iFrame "#".
+          iSplitL ""; first done. iRight. iExists false. iFrame "#".
+          iSplitL ""; first done. by iLeft.
+        }
+        iModIntro.
+        wp_apply (release_spec lockN #mu_ptr _ with "[-Hreply HPost]"); try iFrame "Hmu Hlocked".
+        { (* Re-establish own_lockserver *)
+          iNext. iExists _, _, _, _, _, _, _; try iFrame; try iFrame "#"; try iFrame "%".
+          iPureIntro.
+          split.
+          {
+            intros.
+            admit.
+          }
+          {
+            intros.
+            admit.
+          }
+        }
+        wp_seq.
+        iApply "HPost".
+        iExists false. iFrame. iFrame "#".
+      + (* Lock not held by anyone *)
+
+(*
+        iApply fupd_wp.
+        iInv M as "HMinner" "HCloseM".
+        iDestruct "HMinner" as (lseq_fi _) "HMinner".
+        iMod (map_update lockArgs.(CID) (lseq_fi, last_reply) (lockArgs.(Seq), false) with "Hmapctx Hptsto") as "(Hmapctx & Hptsto)".
+        rewrite (map_insert_zip_with pair _ _ lockArgs.(CID) _ _).
+        iMod ("HCloseM" with "[Hptsto]") as "_".
+        { iModIntro.
+          unfold CallTryLock_inv.
+          iExists lockArgs.(Seq).
+          admit. }
+        iModIntro.
+        wp_seq.
+        wp_loadField.
+        wp_apply (release_spec lockN #mu_ptr _ with "[-Hreply HPost]"); try iFrame "Hmu Hlocked".
+        { (* Estanlish own_lockserver *)
+          iNext. iFrame.
+          iExists _, _, _, _, _, _; iFrame.
+        }
+        wp_seq. iApply ("HPost").
+        iExists false. iFrame. by iRight.
+      + (* Lock not held by anyone *)
+        wp_pures. wp_storeField. repeat wp_loadField.
       wp_apply (wp_MapInsert _ _ locksM _ true #true with "HlocksMap"); first eauto; iIntros "HlocksMap".
       wp_seq. repeat wp_loadField.
       wp_apply (wp_MapInsert _ _ lastReplyM _ true #true with "HlastReplyMap"); first eauto; iIntros "HlastReplyMap".
@@ -300,7 +408,7 @@ Proof.
     wp_pures.
     iApply "HPost". by iLeft.
   }
-*)
+*)*)
 Admitted.
 
 (*
